src/Init/Grind/Tactics.lean
@@ -7,8 +7,19 @@ prelude
 import Init.Tactics
 
 namespace Lean.Grind
+/--
+The configuration for `grind`.
+Passed to `grind` using, for example, the `grind (config := { eager := true })` syntax.
+-/
+structure Config where
+  /--
+  When `eager` is true (default: `false`), `grind` eagerly splits `if-then-else` and `match`
+  expressions.
+  -/
+  eager : Bool := false
+  deriving Inhabited, BEq
+
 /-!
 `grind` tactic and related tactics.
 -/
-
 end Lean.Grind
