src/Lean/Meta/Tactic/Grind.lean
@@ -11,3 +11,4 @@ import Lean.Meta.Tactic.Grind.Preprocessor
 import Lean.Meta.Tactic.Grind.Util
 import Lean.Meta.Tactic.Grind.Cases
 import Lean.Meta.Tactic.Grind.Injection
+import Lean.Meta.Tactic.Grind.Core
