src/Lean/Meta/Tactic/Grind/Types.lean
@@ -11,6 +11,47 @@ import Lean.Meta.Canonicalizer
 import Lean.Meta.Tactic.Util
 
 namespace Lean.Meta.Grind
+
+structure Context where
+  mainDeclName : Name
+
+structure State where
+  canon      : Canonicalizer.State := {}
+  /-- `ShareCommon` (aka `Hashconsing`) state. -/
+  scState    : ShareCommon.State.{0} ShareCommon.objectFactory := ShareCommon.State.mk _
+  /-- Next index for creating auxiliary theorems. -/
+  nextThmIdx : Nat := 1
+
+abbrev GrindM := ReaderT Context $ StateRefT State MetaM
+
+@[inline] def GrindM.run (x : GrindM α) (mainDeclName : Name) : MetaM α :=
+  x { mainDeclName } |>.run' {}
+
+def abstractNestedProofs (e : Expr) : GrindM Expr := do
+  let nextIdx := (← get).nextThmIdx
+  let (e, s') ← AbstractNestedProofs.visit e |>.run { baseName := (← read).mainDeclName } |>.run |>.run { nextIdx }
+  modify fun s => { s with nextThmIdx := s'.nextIdx }
+  return e
+
+def shareCommon (e : Expr) : GrindM Expr := do
+  modifyGet fun { canon, scState, nextThmIdx } =>
+    let (e, scState) := ShareCommon.State.shareCommon scState e
+    (e, { canon, scState, nextThmIdx })
+
+def canon (e : Expr) : GrindM Expr := do
+  let canonS ← modifyGet fun s => (s.canon, { s with canon := {} })
+  let (e, canonS) ← Canonicalizer.CanonM.run (canonRec e) (s := canonS)
+  modify fun s => { s with canon := canonS }
+  return e
+where
+  canonRec (e : Expr) : CanonM Expr := do
+    let post (e : Expr) : CanonM TransformStep := do
+      if e.isApp then
+        return .done (← Meta.canon e)
+      else
+        return .done e
+    transform e post
+
 /--
 Stores information for a node in the egraph.
 Each internalized expression `e` has an `ENode` associated with it.
@@ -43,6 +84,9 @@ structure ENode where
   on heterogeneous equality.
   -/
   heqProofs : Bool := false
+  generation : Nat := 0
+  /-- Modification time -/
+  mt : Nat := 0
   -- TODO: see Lean 3 implementation
 
 structure Clause where
@@ -53,58 +97,57 @@ structure Clause where
 def mkInputClause (fvarId : FVarId) : MetaM Clause :=
   return { expr := (← fvarId.getType), proof := mkFVar fvarId }
 
-structure Goal where
-  mvarId  : MVarId
-  clauses : PArray Clause := {}
-  enodes  : PHashMap UInt64 ENode := {}
-  -- TODO: occurrences for propagation, etc
-  deriving Inhabited
+structure NewEq where
+  lhs   : Expr
+  rhs   : Expr
+  proof : Expr
+  isHEq : Bool
 
-def mkGoal (mvarId : MVarId) : Goal :=
-  { mvarId }
+structure Goal where
+  mvarId       : MVarId
+  clauses      : PArray Clause := {}
+  enodes       : PHashMap USize ENode := {}
+  newEqs       : Array NewEq := #[]
+  /-- `inconsistent := true` if `ENode`s for `True` and `False` are in the same equivalence class. -/
+  inconsistent : Bool := false
+  /-- Goal modification time. -/
+  gmt          : Nat := 0
+  deriving Inhabited
 
 def Goal.admit (goal : Goal) : MetaM Unit :=
   goal.mvarId.admit
 
-structure Context where
-  mainDeclName : Name
+abbrev GoalM := StateRefT Goal GrindM
 
-structure State where
-  canon      : Canonicalizer.State := {}
-  /-- `ShareCommon` (aka `Hashconsing`) state. -/
-  scState    : ShareCommon.State.{0} ShareCommon.objectFactory := ShareCommon.State.mk _
-  /-- Next index for creating auxiliary theorems. -/
-  nextThmIdx : Nat := 1
-  goals      : PArray Goal := {}
+@[inline] def GoalM.run (goal : Goal) (x : GoalM α) : GrindM (α × Goal) :=
+  StateRefT'.run x goal
 
-abbrev GrindM := ReaderT Context $ StateRefT State MetaM
+@[inline] def GoalM.run' (goal : Goal) (x : GoalM Unit) : GrindM Goal :=
+  StateRefT'.run' (x *> get) goal
 
-def GrindM.run (x : GrindM α) (mainDeclName : Name) : MetaM α :=
-  x { mainDeclName } |>.run' {}
+/--
+Returns `some n` if `e` has already been "internalized" into the
+Otherwise, returns `none`s.
+-/
+def getENode? (e : Expr) : GoalM (Option ENode) :=
+  return (← get).enodes.find? (unsafe ptrAddrUnsafe e)
 
-def abstractNestedProofs (e : Expr) : GrindM Expr := do
-  let nextIdx := (← get).nextThmIdx
-  let (e, s') ← AbstractNestedProofs.visit e |>.run { baseName := (← read).mainDeclName } |>.run |>.run { nextIdx }
-  modify fun s => { s with nextThmIdx := s'.nextIdx }
-  return e
+def setENode (e : Expr) (n : ENode) : GoalM Unit :=
+  modify fun s => { s with enodes := s.enodes.insert (unsafe ptrAddrUnsafe e) n }
 
-def shareCommon (e : Expr) : GrindM Expr := do
-  modifyGet fun { canon, scState, nextThmIdx, goals } =>
-    let (e, scState) := ShareCommon.State.shareCommon scState e
-    (e, { canon, scState, nextThmIdx, goals })
+def mkENodeCore (e : Expr) (interpreted ctor : Bool) (generation : Nat) : GoalM Unit := do
+  setENode e {
+    next := e, root := e, cgRoot := e, size := 1
+    flipped := false
+    heqProofs := false
+    hasLambdas := e.isLambda
+    mt := (← get).gmt
+    interpreted, ctor, generation
+  }
 
-def canon (e : Expr) : GrindM Expr := do
-  let canonS ← modifyGet fun s => (s.canon, { s with canon := {} })
-  let (e, canonS) ← Canonicalizer.CanonM.run (canonRec e) (s := canonS)
-  modify fun s => { s with canon := canonS }
-  return e
-where
-  canonRec (e : Expr) : CanonM Expr := do
-    let post (e : Expr) : CanonM TransformStep := do
-      if e.isApp then
-        return .done (← Meta.canon e)
-      else
-        return .done e
-    transform e post
+def mkGoal (mvarId : MVarId) : GrindM Goal := do
+  GoalM.run' { mvarId } do
+    mkENodeCore (← shareCommon (mkConst ``True)) (interpreted := true) (ctor := false) (generation := 0)
+    mkENodeCore (← shareCommon (mkConst ``False)) (interpreted := true) (ctor := false) (generation := 0)
 
 end Lean.Meta.Grind
